Ex2.dfy
@@ -1,17 +1,3 @@
-function noRepetitionF(arr : seq<nat>) : bool
-{
-  if (|arr| == 0) then true
-  else if (existsInArray(arr[1..], arr[0])) then false
-  else noRepetitionF(arr[1..])
-}
-
-function existsInArray(arr : seq<nat>, v : nat) : bool
-{
-  if (|arr| == 0) then false
-  else if (arr[0] == v) then true
-  else existsInArray(arr[1..], v)
-}
-
 method noRepetitionsQuadratic(arr : array<nat>) returns (b: bool) 
   ensures b ==> forall i, j :: 0 <= i < arr.Length && 0 <= j < arr.Length && i != j ==> arr[i] != arr[j]
   ensures !b ==> exists i, j :: 0 <= i < arr.Length && 0 <= j < arr.Length && i != j && arr[i] == arr[j]
@@ -42,10 +28,52 @@ method noRepetitionsQuadratic(arr : array<nat>) returns (b: bool)
   }
 }
 
-
-
-
-method noRepetitionsLinear(arr : array<nat>) returns (b: bool) 
+method Max(nat1 : nat, nat2 : nat) returns (z: nat)
+ensures nat1 > nat2 ==> z == nat1
+ensures nat2 >= nat1 ==> z == nat2
 {
+  if (nat1 > nat2){
+    z := nat1;
+  }
+  else {
+    z := nat2;
+  }
+  return;
+} 
 
+
+method noRepetitionsLinear(arr : array<nat>) returns (b: bool)
+  ensures b ==> forall i, j :: 0 <= i < arr.Length && 0 <= j < arr.Length && i != j ==> arr[i] != arr[j]
+  ensures !b ==> exists i, j :: 0 <= i < arr.Length && 0 <= j < arr.Length && i != j && arr[i] == arr[j]
+{
+  var max : nat := 0;
+  var i := 0;
+  
+  while (i < arr.Length)
+  invariant 0 <= i <= arr.Length
+  invariant forall k :: 0 <= k < i ==> arr[k] <=  max
+  {
+    max := Max(max, arr[i]);
+    i := i + 1;
+  }
+
+  var table := new bool[max + 1] (_ => false);
+
+  i:= 0;
+  b := true;
+  while (i < arr.Length)
+  invariant 0 <= i <= arr.Length
+  invariant forall k :: 0 <= k < i ==> table[arr[k]]
+  invariant forall k :: (0 <= k <= max && table[k]) ==> (exists j :: 0 <= j < arr.Length && arr[j] == k)
+  invariant forall k, m :: 0 <= k < i && 0 <= m < i && k != m ==> arr[k] != arr[m]
+  {
+    if (table[arr[i]]) {
+      b := false;
+      return;
+    }
+    table[arr[i]] := true;
+    i := i + 1;
+  }
+  b := true;
+  return;
 }
